add single-node failstop adequacy theorem

src/goose_lang/recovery_adequacy.v
@@ -6,19 +6,19 @@ From Perennial.goose_lang Require Export recovery_lifting.
 From Perennial.goose_lang Require Import typing adequacy lang crash_borrow.
 Set Default Proof Using "Type".
 
-Theorem goose_recv_adequacy `{ffi_sem: ffi_semantics} `{!ffi_interp ffi} {Hffi_adequacy:ffi_interp_adequacy} Σ `{hPre: !gooseGpreS Σ} s e r σ g φ φr φinv Φinv n :
+Theorem goose_recv_adequacy `{ffi_sem: ffi_semantics} `{!ffi_interp ffi} {Hffi_adequacy:ffi_interp_adequacy} Σ `{hPre: !gooseGpreS Σ} s e r σ g φ φr φinv n :
   ffi_initgP g.(global_world) → ffi_initP σ.(world) g.(global_world) →
-  (∀ `(Hheap : !heapGS Σ),
-     ⊢ (ffi_global_start goose_ffiGlobalGS g.(global_world) -∗
-        ffi_local_start goose_ffiLocalGS σ.(world) -∗
-        trace_frag σ.(trace) -∗
-        oracle_frag σ.(oracle) -∗
-        pre_borrowN n ={⊤}=∗
-        □ (∀ σ nt, state_interp σ nt -∗ |NC={⊤, ∅}=> ⌜ φinv σ ⌝) ∗
-        □ (∀ hL : gooseLocalGS Σ,
-            let hG := HeapGS _ _ hL in
-            Φinv hG -∗ □ ∀ σ nt, state_interp σ nt -∗ |NC={⊤, ∅}=> ⌜ φinv σ ⌝) ∗
-        wpr s ⊤ e r (λ v, ⌜φ v⌝) (Φinv) (λ _ v, ⌜φr v⌝))) →
+  (∀ `(Hheap : !heapGS Σ), ∃ Φinv,
+     ⊢ ffi_global_start goose_ffiGlobalGS g.(global_world) -∗
+       ffi_local_start goose_ffiLocalGS σ.(world) -∗
+       trace_frag σ.(trace) -∗
+       oracle_frag σ.(oracle) -∗
+       pre_borrowN n ={⊤}=∗
+       □ (∀ σ nt, state_interp σ nt -∗ |NC={⊤, ∅}=> ⌜ φinv σ ⌝) ∗
+       □ (∀ hL : gooseLocalGS Σ,
+           let hG := HeapGS _ _ hL in
+           Φinv hG -∗ □ ∀ σ nt, state_interp σ nt -∗ |NC={⊤, ∅}=> ⌜ φinv σ ⌝) ∗
+       wpr s ⊤ e r (λ v, ⌜φ v⌝) (Φinv) (λ _ v, ⌜φr v⌝)) →
   recv_adequate (CS := goose_crash_lang) s e r σ g (λ v _ _, φ v) (λ v _ _, φr v) (λ σ _, φinv σ).
 Proof.
   intros Hinit Hinitg Hwp.
@@ -37,12 +37,12 @@ Proof.
   (* TODO(RJ): reformulate init lemmas to better match what we need here. *)
   set (hG := GooseGlobalGS _ _ proph_names (creditGS_update_pre _ _ name_credit) ffi_namesg).
   set (hL := GooseLocalGS Σ Hc ffi_names (na_heapGS_update_pre _ name_na_heap) (traceGS_update_pre Σ _ name_trace)).
+  destruct (Hwp (HeapGS _ hG hL)) as [Φinv Hwp']. clear Hwp.
   iExists state_interp, global_state_interp, fork_post.
   iExists _, _.
-
   iExists ((λ Hinv hGen, ∃ hL:gooseLocalGS Σ, ⌜hGen = goose_generationGS (L:=hL)⌝ ∗ Φinv (HeapGS _ _ hL)))%I.
   iDestruct (@cred_frag_to_pre_borrowN _ _ _ _ _ hG n with "Hpre") as "Hpre".
-  iMod (Hwp (HeapGS _ hG hL) with "[$] [$] [$] [$] [$]") as "(#H1&#H2&Hwp)".
+  iMod (Hwp' with "[$] [$] [$] [$] [$]") as "(#H1&#H2&Hwp)".
   iModIntro.
   iSplitR.
   { iModIntro. iIntros (??) "Hσ".
@@ -60,3 +60,45 @@ Proof.
   iSplit; first by eauto.
   iIntros (? v) "(% & % & $)". done.
 Qed.
+
+Section failstop.
+
+Context `{ffi_sem: ffi_semantics} `{!ffi_interp ffi} {Hffi_adequacy:ffi_interp_adequacy}.
+
+(* We can model failstop execution by just having the restart thread be a trivial program that just halts.
+   Thus, the machine "restarts" after a crash but it does not do anything. *)
+Definition adequate_failstop (e: expr) (σ: state) (g: global_state)
+    (φpost : val → state → global_state → Prop) :=
+  recv_adequate (CS := goose_crash_lang) NotStuck e (of_val #()) σ g φpost (λ _ _ _, True) (λ _ _, True).
+
+(* Like above, but, for failstop execution one only needs to prove a wp, not a
+wpr. Due to that, no φinv is supported (since after the crash σ changed so
+[φinv σ] no longer has any reason to hold). *)
+Theorem goose_recv_adequacy_failstop
+        Σ `{hPre: !gooseGpreS Σ} (e: expr) (σ: state) (g: global_state) φpost :
+  ffi_initgP g.(global_world) → ffi_initP σ.(world) g.(global_world) →
+  (∀ `(Hheap : !heapGS Σ),
+    ⊢ ffi_global_start goose_ffiGlobalGS g.(global_world) -∗
+      ffi_local_start goose_ffiLocalGS σ.(world) ={⊤}=∗
+      WP e @ ⊤ {{ v, ⌜φpost v⌝ }}) →
+  adequate_failstop e σ g (λ v _ _, φpost v).
+Proof.
+  intros Hinitg Hinit Hwp. eapply goose_recv_adequacy with (n:=0%nat); [done..|].
+  intros hHeap. exists (λ _, True)%I.
+  iIntros "Hstartg Hstart _ _ _".
+  iMod (Hwp with "Hstartg Hstart") as "Hwp". iModIntro.
+  iSplitR.
+  { iIntros "!> * _". iApply ncfupd_mask_intro; auto. }
+  iSplitR.
+  { do 2 iIntros "!> * _". iApply ncfupd_mask_intro; auto. }
+  iApply (idempotence_wpr _ _ _ _ _ _ _ (λ _, True%I) with "[Hwp] []").
+  { iApply wp_wpc. eauto. }
+  { iModIntro. iIntros (????) "_".
+    iModIntro.
+    rewrite /crash_modality.post_crash.
+    iIntros (???) "H". iModIntro; iFrame. iIntros "H". iSplit; first auto.
+    iApply wpc_value; eauto.
+  }
+Qed.
+
+End failstop.
